modified:   coq/sf/Makefile 	new file:   coq/sf/apply.v 	modified:   coq/sf/church.v 	new file:   haskell/OverlappingInstances.hs 	new file:   haskell/OverlappingInstances2.hs 	new file:   haskell/TypeSynonymInstances.hs 	modified:   haskell/foldl.hs 	new file:   haskell/sprint.hs

haskell/OverlappingInstances.hs
@@ -1,0 +1,23 @@
+{-# LANGUAGE    MultiParamTypeClasses, 
+                FlexibleInstances,
+                OverlappingInstances -- deprecated
+#-}
+
+-- MultiParamTypeClasses needed here
+class MyClass a b where
+    fn :: (a,b)
+
+-- FlexibleInstances needed here
+instance MyClass Int b where
+    fn = error "b"
+
+-- fine , but will need OverlappingInstances if 'fn' called
+instance MyClass a Int where
+    fn = error "a"
+
+instance MyClass Int Int where
+    fn = error "c"
+
+example :: (Int,Int)
+example = fn 
+
