haskell/TypeSynonymInstances.hs
@@ -1,0 +1,12 @@
+{-# LANGUAGE FlexibleInstances, TypeSynonymInstances  #-}
+
+type IntList = [Int]
+
+class MyClass a
+
+-- FlexibleInstances required
+--instance MyClass [Int]
+
+-- don't get it
+instance MyClass IntList
+
