haskell/foldl.hs
@@ -17,6 +17,7 @@ foldl' op acc (x:xs)  = let new = op acc x  -- will force evaluation using seq
 
 
 -- seriously quicker with strict evaluation (foldl')
+-- even with -O2 compile option
 main :: IO ()
 main = do
   putStrLn $ show $ foldl' (+) 0 [1..5000000]
