haskell/sprint.hs
@@ -1,0 +1,4 @@
+-- use ghci :sprint x to see evaluation status of x
+
+a = [1..] :: [Integer]
+b = map (+1) a
